Veritas.Verifier.Global.fst
@@ -112,10 +112,10 @@ let add_set_map_inv (gl: verifiable_log) (j: seq_index (g_add_seq gl)):
   (ii: sseq_index gl {is_blum_add (indexss gl ii) /\ 
                       add_set_map gl ii = j}) = admit()
 
-let lemma_add_set_map_into (gl: verifiable_log) (ii1 ii2: sseq_index gl):
-  Lemma (requires (is_blum_add (indexss gl ii1) /\
-                   is_blum_add (indexss gl ii2)))
-        (ensures (ii1 <> ii2 ==> add_set_map gl ii1 <> add_set_map gl ii2)) = admit()
+let lemma_add_set_map_inv (gl: verifiable_log)(ii: sseq_index gl {is_blum_add (indexss gl ii)}):
+  Lemma (requires True)
+        (ensures (add_set_map_inv gl (add_set_map gl ii) = ii))
+        [SMTPat (add_set_map gl ii)] = admit()
 
 let rec g_evict_seq_aux (gl: verifiable_log):
   Tot (seq (ms_hashfn_dom))
