Veritas.Verifier.Global.fsti
@@ -66,10 +66,10 @@ val add_set_map_inv (gl: verifiable_log) (j: seq_index (g_add_seq gl)):
   (ii: sseq_index gl {is_blum_add (indexss gl ii) /\ 
                       add_set_map gl ii = j})
 
-val lemma_add_set_map_into (gl: verifiable_log) (ii1 ii2: sseq_index gl):
-  Lemma (requires (is_blum_add (indexss gl ii1) /\
-                   is_blum_add (indexss gl ii2)))
-        (ensures (ii1 <> ii2 ==> add_set_map gl ii1 <> add_set_map gl ii2))
+val lemma_add_set_map_inv (gl: verifiable_log)(ii: sseq_index gl {is_blum_add (indexss gl ii)}):
+  Lemma (requires True)
+        (ensures (add_set_map_inv gl (add_set_map gl ii) = ii))
+        [SMTPat (add_set_map gl ii)]
 
 (* a single sequence containing all the blum evicts *)
 val g_evict_seq (gl: verifiable_log): seq ms_hashfn_dom 
